promising-arm/Common.v
@@ -1,0 +1,150 @@
+(** This file contains common definition and automation helpers that are use in
+    the rest of this development.
+
+    It contains automation helpers, some patching to get multiple library to
+    interact correctly with each other and various utility definitions. *)
+
+From Hammer Require Export Tactics.
+From RecordUpdate Require Export RecordSet.
+From stdpp Require Export base strings.
+Require Export bbv.Word.
+
+Require Import Sail.Base.
+
+Require Import PRelations.
+
+
+(** Functional pipe notation.
+
+    TODO figure out a correct parsing level. Currently is just below relation so
+    that a = b |> f will be parsed as a = (b |> f). *)
+Notation "v |> f" := (f v) (at level 69, only parsing, left associativity).
+
+
+
+(********** Boolean reflection **********)
+
+(* This is a hack to make CoqHammer boolean reflection use the Is_true coercion
+    from stdpp*)
+
+(* Using a plain Require and not Require Import is critical to not import the
+   is_true coercion since stdpp already uses the Is_true coercion. *)
+From Hammer Require Reflect.
+
+Tactic Notation "breflect" :=
+  try rewrite_strat topdown hints brefl.
+
+Tactic Notation "breflect" "in" hyp(H) :=
+  try rewrite_strat topdown hints brefl in H.
+
+Tactic Notation "breflect" "in" "*" :=
+  breflect;
+  repeat match goal with
+         | [H : _ |- _ ] => rewrite_strat topdown hints brefl in H
+         end.
+
+(* Convert the normal coercion to the is_true one that CoqHammer expects. *)
+Lemma true_is_true (b : bool) : b <-> is_true b.
+  Proof. sauto lq:on. Qed.
+Hint Rewrite -> true_is_true : brefl.
+Hint Rewrite <- true_is_true : breif.
+
+
+(** existsb boolean reflection *)
+Lemma existsb_exists' (A : Type) (f : A → bool) (l : list A):
+  is_true (existsb f l) ↔ (∃ x : A, In x l ∧ is_true(f x)).
+Proof. unfold is_true. apply existsb_exists. Qed.
+Hint Rewrite existsb_exists' : brefl.
+
+
+
+
+(********** List automation **********)
+
+(** Automation for list simplifications *)
+Tactic Notation "list_simp" "in" "|-*" :=
+  rewrite_strat topdown hints list.
+
+Tactic Notation "list_simp" "in" hyp(H) :=
+  rewrite_strat topdown hints list in H.
+
+Tactic Notation "list_simp" :=
+  progress (try list_simp in |-*;
+  repeat match goal with
+         | [H : _ |- _ ] => rewrite_strat topdown hints list in H
+         end).
+
+Hint Rewrite in_app_iff : list.
+Arguments elem_of_list_In : clear implicits.
+Hint Rewrite elem_of_list_In : list.
+Arguments list_subseteq _ _ _ /.
+Hint Rewrite Forall_forall : list.
+
+Global Hint Resolve in_map : list.
+
+
+
+
+(********** Decidable equality **********)
+
+(** Decidable equality notation that use the EqDecision type class from stdpp*)
+Notation "x == y" := (bool_decide (x = y)) (at level 70, no associativity).
+
+(** Boolean reflection of decidable equality. *)
+Lemma bool_decide_is_true (P : Prop) {dec : Decision P} :
+  is_true (bool_decide P) <-> P.
+Proof. unfold is_true. apply bool_decide_eq_true. Qed.
+Hint Rewrite bool_decide_is_true : brefl.
+
+(* Interface Equality decision for words (from bbv) *)
+Global Instance word_eq_dec n : EqDecision (word n).
+Proof.
+  unfold EqDecision.
+  unfold Decision.
+  auto using weq.
+Defined.
+
+(** Convert automatical a Decidable instance (Coq standard library) to
+    a Decision instance (stdpp)
+
+    TODO: Decide (no pun intended) if we actually want to use Decidable or
+    Decision in this development. *)
+Global Instance Decidable_to_Decision P `{dec : Decidable P} : Decision P.
+Proof.
+  (* sauto lq:on dep:on works, but since this is a Defined and noq a Qed.
+     I went for a manual proof that prooduces a simpler term. *)
+  unfold Decision.
+  destruct dec as [p Spec].
+  destruct p.
+  - left.
+    apply Spec.
+    reflexivity.
+  - right.
+    intro.
+    apply Spec in H.
+    inversion H.
+Defined.
+
+
+
+
+(********** Utility functions **********)
+
+(** Update a function at a specific value *)
+Definition fun_add {A B} {_: EqDecision A} (k : A) (v : B) (f : A -> B) :=
+  fun x : A => if k == x then v else f x.
+
+
+(** A list_remove version that uses the EqDecision typeclass *)
+Definition list_remove `{EqDecision A} :=
+  List.remove (decide_rel (=@{A})).
+
+
+(** I couldn't find this in the standard library but there should be something
+somewhere. I can't be the first one to need that.*)
+Fixpoint list_set {A} (n : nat) (v : A) (l : list A) :=
+  match l, n with
+  | nil, _ => nil
+  | h :: t, 0%nat => v :: t
+  | h :: t, S m => h :: (list_set m v t)
+  end.
