promising-arm/Exec.v
@@ -1,0 +1,298 @@
+(* This file defines an execution monad for the model.
+
+   It is not intended to be Imported as name are not qualified.
+
+   The execution model is Either a named error or a lists of possible outputs.
+   This is used to represent non-deterministic but computational execution that
+   may fail.
+
+   Getting a Results l, means that all path from the initial state have been
+   computed and all the results are in l and none of them are errors.
+
+   Getting an Error e, means that there is one non-deterministic path that
+   reaches that error. All other possible outcome are specified.
+
+   In the case of this model, an Error means a behavior not supported by the
+   model. In particular, since processor exceptions are not supported, any
+   invalid code that would trigger them will make the whole execution return
+   an error with hopefully a descriptive message. *)
+
+Require Import Common.
+
+
+
+
+(********** Definition and utility functions **********)
+
+Inductive t (E A : Type) : Type :=
+| Error : E -> t E A
+| Results : list A -> t E A.
+Arguments Error {_ _} _.
+Arguments Results {_ _} _.
+
+(** Means that this execution has no output and may be safely discarded.*)
+Notation discard := (Results []).
+
+(** Monadic return *)
+Definition ret {E A} (a : A) : t E A := Results [a].
+
+(** Takes an option but convert None into an error *)
+Definition error_none {E A} (e : E) : option A -> t E A :=
+  from_option ret (Error e).
+
+(** Takes an option but convert None into a discard *)
+Definition discard_none {E A} : option A -> t E A :=
+  from_option ret discard.
+
+(** Returns an error if the condition is met *)
+Definition fail_if {E} (b : bool) (e : E) : t E () :=
+  if b then Error e else ret ().
+
+(** Discards the execution if the condition is not met *)
+Definition assert {E} (b : bool) : t E () :=
+  if b then ret () else discard.
+
+(** Maps the error to another error type. *)
+Definition map_error {E E' A} (f : E -> E') (e : t E A) : t E' A :=
+  match e with
+  | Error err => Error (f err)
+  | Results l => Results l
+  end.
+
+(** Merge the results of two executions *)
+Definition merge {E A} (e1 e2 : t E A) :=
+  match e1 with
+  | Error e => Error e
+  | Results l =>
+      match e2 with
+      | Error e => Error e
+      | Results l' => Results (l ++ l')
+      end
+  end.
+
+
+(********** Monad instance **********)
+
+Global Instance mret_inst {E} : MRet (t E) := { mret A := ret }.
+
+Global Instance mbind_inst {E} : MBind (t E) :=
+  { mbind _ _ f x :=
+    match x with
+    | Error e => Error e
+    | Results l => foldl merge discard (map f l)
+    end
+  }.
+
+Global Instance fmap_inst {E} : FMap (t E) :=
+  { fmap _ _  f x :=
+    match x with
+    | Error e => Error e
+    | Results l => Results (map f l)
+    end }.
+
+
+
+(********** Simplification lemmas **********)
+
+Lemma mbind_ret E A B (x : A) (f : A -> t E B) : (ret x ≫= f) = f x.
+Proof. hauto lq:on. Qed.
+Hint Rewrite mbind_ret : exec.
+
+Lemma mbind_error (E A B : Type) e (f : A -> t E B) : Error e ≫= f = Error e.
+Proof. done. Qed.
+Hint Rewrite mbind_error : exec.
+
+Lemma mbind_discard E A B (f : A -> t E B) : discard ≫= f = discard.
+Proof. done. Qed.
+Hint Rewrite mbind_discard : exec.
+
+Lemma merge_error E A s (e : t E A):
+  merge (Error s) e = Error s.
+Proof. done. Qed.
+Hint Rewrite merge_error : exec.
+
+Lemma foldl_merge_error E A s (l : list (t E A)):
+  foldl merge (Error s) l = Error s.
+Proof. by induction l. Qed.
+Hint Rewrite foldl_merge_error : exec.
+
+Lemma merge_discard E A (e : t E A) : merge discard e = e.
+Proof. by destruct e. Qed.
+Hint Rewrite merge_discard : exec.
+
+Lemma mbind_cons E A B (x : A) (l : list A) (f : A -> t E B):
+  Results (x :: l) ≫= f =
+    merge (f x) (Results l ≫= f).
+  simpl.
+  destruct (f x) as [|lx]; [ by autorewrite with exec| clear x].
+  - generalize dependent lx.
+    induction (map f l) as [| y lt]; hauto use: app_assoc inv:t db:exec,list.
+Qed.
+Hint Rewrite mbind_cons : exec.
+
+
+(********** Predicate on the results **********)
+
+(** Describe an non-error execution *)
+Inductive has_results {E A} : t E A -> Prop :=
+| HResults l : has_results (Results l).
+Global Hint Constructors has_results : exec.
+
+(** Describe the fact that an execution is successful and contains the
+    specified value *)
+Inductive In {E A} (x : A) : t E A -> Prop :=
+| InIn l : List.In x l -> In x (Results l).
+Global Hint Constructors In : exec.
+
+
+Lemma in_has_results E A (e : t E A) x : In x e -> has_results e.
+Proof. sauto lq:on. Qed.
+Global Hint Resolve in_has_results : exec.
+
+
+
+
+(********** Simplification with the predicates **********)
+
+Lemma has_results_error E A err: has_results (Error err : t E A) <-> False.
+Proof. sauto. Qed.
+Hint Rewrite has_results_error : exec.
+
+Lemma in_error E A (err : E) (x : A) : In x (Error err) <-> False.
+Proof. sauto. Qed.
+Hint Rewrite in_error : exec.
+
+Lemma in_discard E A (x : A) : In x (discard : t E A) <-> False.
+Proof. sauto. Qed.
+Hint Rewrite in_discard: exec.
+
+Lemma has_results_results E A l : has_results (Results l : t E A) <-> True.
+Proof. sauto. Qed.
+Hint Rewrite has_results_results : exec.
+
+Lemma in_results E A (x : A) l : In x (Results l : t E A) <-> List.In x l.
+Proof. sauto. Qed.
+Hint Rewrite in_results : exec.
+
+Lemma has_results_merge E A (e e' : t E A) :
+  has_results (merge e e') <-> has_results e /\ has_results e'.
+Proof. destruct e; destruct e'; hauto inv:has_results db:list,exec. Qed.
+Hint Rewrite has_results_merge : exec.
+
+Lemma in_merge E A (e e' : t E A) x :
+  In x (merge e e') <->
+    (In x e /\ has_results e') \/ (has_results e /\ In x e').
+Proof. destruct e; destruct e'; sauto db:list. Qed.
+Hint Rewrite in_merge : exec.
+
+Lemma in_ret E A (x y :A) : In x (ret y : t E A) <-> x = y.
+Proof. sauto. Qed.
+Hint Rewrite in_ret : exec.
+
+Lemma has_results_error_none E A (err : E) opt :
+  has_results (error_none err opt) <-> exists x : A, opt = Some x.
+Proof. sauto q:on rew:off. Qed.
+Hint Rewrite has_results_error_none : exec.
+
+Lemma in_error_none E A (x : A) (err : E) opt :
+  In x (error_none err opt) <-> opt = Some x.
+Proof. sauto q:on rew:off. Qed.
+Hint Rewrite in_error_none : exec.
+
+Lemma has_results_map_error E E' A (e : t E A) (f : E -> E') :
+  has_results (map_error f e) <-> has_results e.
+Proof. sauto q:on rew:off. Qed.
+Hint Rewrite has_results_map_error : exec.
+
+Lemma in_map_error E E' A (x : A) (e : t E A) (f : E -> E') :
+  In x (map_error f e) <-> In x e.
+Proof. sauto q:on rew:off. Qed.
+Hint Rewrite in_map_error : exec.
+
+Lemma has_results_results_mbind E A B (l : list A) (f : A -> t E B):
+  has_results (Results l ≫= f) <-> List.Forall (fun z => has_results (f z)) l.
+Proof. induction l; hauto inv:List.Forall l:on db:exec. Qed.
+
+
+Lemma in_results_mbind E A B (x : B) (l : list A) (f: A -> t E B) :
+  In x (Results l ≫= f) <->
+    (exists y : A, List.In y l /\ In x (f y)) /\
+      List.Forall (fun z => has_results (f z)) l.
+Proof.
+  induction l.
+  - hauto lq:on db:exec.
+  - autorewrite with exec.
+    rewrite has_results_results_mbind.
+    hauto lq:on db:exec, list.
+Qed.
+
+Lemma has_results_mbind E A B (e : t E A) (f : A -> t E B):
+  has_results (e ≫= f) <->
+    has_results e /\ forall z, In z e -> has_results (f z).
+Proof.
+  destruct e.
+  - hauto inv:has_results.
+  - rewrite has_results_results_mbind.
+    hauto db:list,exec.
+Qed.
+Hint Rewrite has_results_mbind : exec.
+
+Lemma in_mbind E A B (x : B) e (f: A -> t E B) :
+  In x (e ≫= f) <-> (exists y : A, In y e /\ In x (f y)) /\
+                    (forall z, In z e -> has_results (f z)).
+Proof.
+  destruct e.
+  - hauto inv:In.
+  - rewrite in_results_mbind.
+    hauto db:list,exec.
+Qed.
+Hint Rewrite in_mbind : exec.
+
+(* This is an optimisation of the previous rewriting rules *)
+Lemma in_error_none_mbind E A B (x : B) (f: A -> t E B) err opt :
+  In x (error_none err opt ≫= f) <-> exists y, opt = Some y /\ In x (f y).
+Proof. hauto db:exec. Qed.
+Hint Rewrite in_error_none_mbind : exec.
+
+
+
+
+(********** Inclusion of execution **********)
+
+(** A execution being included in another means that a success in the
+    first implies a success in the second and all elements in the first
+    are also in the second *)
+Definition Incl {E E' A B} (f : A -> B) (e : t E A) (e' : t E' B) : Prop :=
+  (has_results e -> has_results e') /\
+    forall x : A, In x e -> In (f x) e'.
+
+Lemma Incl_In E A B (e : t E A) (e' : t E B) x f :
+  Incl f e e' -> In x e -> In (f x) e'.
+Proof. firstorder. Qed.
+
+Lemma Incl_has_results E A (e e' : t E A) f :
+  Incl f e e' -> has_results e -> has_results e'.
+Proof. firstorder. Qed.
+
+
+
+
+(********** Tactics **********)
+
+(** This module is intended to be imported and provides tactics to be used
+    to deal with the exec monad *)
+Module Tactics.
+
+  Tactic Notation "exec_simp" "in" "|-*" :=
+    rewrite_strat topdown hints exec.
+
+  Tactic Notation "exec_simp" "in" hyp(H) :=
+    rewrite_strat topdown hints exec in H.
+
+  Tactic Notation "exec_simp" :=
+    progress
+      (repeat exec_simp in |-*;
+            repeat match goal with
+                   | [H : _ |- _ ] => rewrite_strat topdown  (repeat hints exec) in H
+                   end).
+End Tactics.
